theories/IL/VarP.v
@@ -1,4 +1,4 @@
-Require Import Var IL.
+Require Import Util Var IL DecSolve Indexwise.
 
 Inductive var_P (P:var -> Prop)
   : stmt -> Prop :=
@@ -30,4 +30,25 @@ Lemma var_P_occurVars (P:var -> Prop) s
 Proof.
   induction 1; unfold For_all in *; intros; simpl in *; cset_tac'.
   eapply list_union_get in H4. destruct H4; dcr; inv_get; cset_tac.
+Qed.
+
+Instance var_P_dec P (DEC:forall x, Computable (P x)) s : Computable (var_P P s).
+Proof.
+  sind s; destruct s.
+  - ensure (P x); ensure (For_all P (Exp.freeVars e));
+    destruct (IH s); dec_solve.
+  - ensure (For_all P (Ops.freeVars e));
+    destruct (IH s1); eauto; [|dec_solve];
+      destruct (IH s2); eauto; dec_solve.
+  - ensure (For_all P (list_union (Ops.freeVars ⊝ Y))); dec_solve.
+  - ensure (For_all P (Ops.freeVars e)); dec_solve.
+  - destruct (IH s); eauto; try dec_solve.
+    assert (Computable (forall n Zs, get F n Zs -> var_P P (snd Zs))). {
+      eapply indexwise_P_dec. intros. eapply IH; eauto.
+    }
+    destruct H; [|dec_solve].
+    assert (Computable (forall n Zs, get F n Zs -> For_all P (of_list (fst Zs)))). {
+      eapply indexwise_P_dec. intros. eauto with typeclass_instances.
+    }
+    destruct H; dec_solve.
 Qed.
